Hs/Metatheory/TypeMatchCompile.lean
@@ -1,0 +1,60 @@
+import Hs.Algorithm
+import Hs.Metatheory.Uniqueness
+import Hs.Metatheory.Weaken
+import Hs.Metatheory.WeakenCompile
+import Hs.Metatheory.Substitution
+import Hs.Metatheory.SubstitutionCompile
+import Hs.Metatheory.Preservation1
+import SystemFD.Algorithm.Soundness2
+
+
+theorem compile_type_match :
+ -- (∀ Γ (h1 h2 : ⊢s Γ), h1 = h2) ->
+ (∀ v, CompileCtxPred v) ->
+ ⊢ Γ' ->
+ (jA : Γ ⊢τ A : `★) ->
+ compile_type Γ A `★ jA = .some A' ->
+ (jA : Γ ⊢τ R : `★) ->
+ compile_type Γ R `★ jR = .some R' ->
+ StableHsTypeMatch Γ A R -> StableTypeMatch Γ' A' R' := by sorry
+
+
+theorem compile_stable_match :
+ -- (∀ Γ (h1 h2 : ⊢s Γ), h1 = h2) ->
+ (∀ v, CompileCtxPred v) ->
+ ⊢ Γ' ->
+ (jA : Γ ⊢τ A : `★) ->
+ compile_type Γ A `★ jA = .some A' ->
+ (jR : Γ ⊢τ R : `★) ->
+ compile_type Γ R `★ jR = .some R' ->
+ StableHsTypeMatch Γ A R -> StableTypeMatch Γ' A' R' := by sorry
+
+
+theorem compile_prefix_match :
+ -- (∀ Γ (h1 h2 : ⊢s Γ), h1 = h2) ->
+ (∀ v, CompileCtxPred v) ->
+ ⊢ Γ' ->
+ (jA : Γ ⊢τ A : `★) ->
+ compile_type Γ A `★ jA = .some A' ->
+ (jR : Γ ⊢τ R : `★) ->
+ compile_type Γ R `★ jR = .some R' ->
+ (jT : Γ ⊢τ T : `★) ->
+ compile_type Γ T `★ jT = .some T' ->
+ PrefixHsTypeMatch Γ A R T -> PrefixTypeMatch Γ' A' R' T' := by sorry
+
+theorem compile_preserves_vhv_types test σtest :
+ (∀ v, CompileCtxPred v) ->
+ ⊢ Γ' ->
+ (jT : Γ ⊢τ T : `★) ->
+ compile_type Γ T `★ jT = .some T' ->
+ HsValidHeadVariable T test ->
+ ValidHeadVariable T' σtest := by sorry
+
+
+theorem compile_preserves_vhv_terms test σtest :
+ (∀ v, CompileCtxPred v) ->
+ ⊢ Γ' ->
+ (jT : Γ ⊢t T : τ) ->
+ compile_term Γ T τ jT = .some T' ->
+ HsValidHeadVariable T test ->
+ ValidHeadVariable T' σtest := by sorry
