Hs/Metatheory/Uniqueness.lean
@@ -186,19 +186,19 @@ intro j; cases j; rfl
 @[simp]
 abbrev TypingJudgmentsUniquessType : (v : HsVariant) -> Ctx HsTerm -> HsJudgmentArgs v -> Prop
 | .term => λ Γ => λ (t, τ) =>
+  (∀ Γ (h1 h2 : ⊢s Γ), h1 = h2) ->
    (j1 : Γ ⊢t t : τ) -> (j2 : Γ ⊢t t : τ) -> j1 = j2
 | _ => λ _ => λ _ => true
 
 theorem terms_have_unique_judgments_lemma :
-  (∀ Γ (h1 h2 : ⊢s Γ), h1 = h2) ->
   HsJudgment v Γ idx -> TypingJudgmentsUniquessType v Γ idx := by
-intro h j; induction j <;> simp at *
-all_goals (intro j1 j2)
-case _ =>
-
+intro j; induction j <;> simp at *
+all_goals (intro h j1 j2)
+case _ h1 h2 vhv j3 ih1 ih2 ih3 =>
   sorry
 case _ =>
-
+  sorry
+case _ =>
   sorry
 case _ => sorry
 case _ => sorry
@@ -206,9 +206,6 @@ case _ => sorry
 case _ => sorry
 case _ => sorry
 case _ => sorry
-case _ => sorry
-
-
 
 theorem terms_have_unique_judgments :
   (∀ Γ (h1 h2 : ⊢s Γ), h1 = h2) ->
@@ -216,4 +213,4 @@ theorem terms_have_unique_judgments :
   (j2 : Γ ⊢t t : k) ->
   j1 = j2 := by
 intro h j1 j2;
-apply terms_have_unique_judgments_lemma h j2 j1 j2;
+apply terms_have_unique_judgments_lemma j2 h j1 j2;
